Stuck on Guess Example. Some instances to handle cases with universe 1 and 0

state/Examples.Guess.fst
@@ -12,32 +12,74 @@ type cmp = | LT | GT | EQ
 instance witnessable_cmp : witnessable cmp = { satisfy = (fun _ _ -> True) }
 instance poly_iface_cmp a3p : poly_iface a3p cmp = { wt = witnessable_cmp }
 
-let post_cond = PolyIface.c3p_hrel
+type player_type a3p =
+  args:((int & int) & (guess: (mk_poly_arrow a3p int cmp))) ->
+  ST int (requires (fun h0 -> inv a3p h0 /\ fst (fst args) < snd (fst args))) (ensures fun h0 r h1 -> inv a3p h1 /\ h0 `hrel a3p` h1)
 
-type player_type =
-  args:((int & int) & (guess: int -> SST cmp (fun _ -> True) (fun h0 r h1 -> post_cond h0 h1))) ->
-  SST int (requires (fun _ -> fst (fst args) < snd (fst args))) (ensures fun h0 r h1 -> post_cond h0 h1)
+type play_guess_type a3p =
+  args:(player_type a3p & (int & (int & int))) ->
+  ST (resexn (bool & int)) (requires fun h0 -> inv a3p h0 /\ fst (snd (snd args)) < fst (snd args) /\ fst (snd args) < snd (snd (snd args))) (ensures fun h0 r h1 -> inv a3p h1 /\ h0 `hrel a3p` h1)
 
-let play_guess (args:player_type & (int & (int & int))) : 
-  SST (bool & int)
-  (requires fun _ -> fst (snd (snd args)) < fst (snd args) /\ fst (snd args) < snd (snd (snd args))) 
-  (ensures fun h0 r h1 -> post_cond h0 h1) =
+val play_guess : play_guess_type c3p
+let play_guess args =
   let player, (pick, (l, r)) = args in
   let counter : mref int (fun v' v'' -> b2t (v' <= v'')) = sst_alloc 0 in
   sst_encapsulate counter;
   witness (contains_pred counter);witness (is_encapsulated counter);
-  let cb (g:int) : SST cmp (fun _ -> True) (fun h0 r h1 -> post_cond h0 h1) = (
+  let cb (g:int) : SST cmp (fun _ -> True) (fun h0 r h1 -> h0 `hrel_c` h1) = (
     recall (contains_pred counter);recall (is_encapsulated counter);
     sst_write counter ((sst_read counter) + 1);
     if g = pick then EQ else if pick < g then LT else GT) in
   let final_guess = player ((l,r),cb) in
-  if pick = final_guess then (true, !counter)
-  else (false, !counter)
+  if pick = final_guess then (Inl (true, !counter))
+  else (Inl (false, !counter))
 
-instance importable_player a3p : safe_importable_to a3p (mk_poly_arrow a3p ((int & int) & (mk_poly_arrow a3p int cmp)) int) Leaf =
-  poly_iface_is_safely_importable a3p _ #(poly_iface_arrow a3p ((int & int) & (mk_poly_arrow a3p int cmp)) int #(
-    poly_iface_pair a3p (int & int) (mk_poly_arrow a3p int cmp) #_ #(poly_iface_arrow a3p int cmp)
-  ) #_)
+open FStar.Tactics
+open FStar.Tactics.Typeclasses
 
-// instance exportable_guess a3p : exportable_from a3p (mk_poly_arrow a3p (player_type & (int & (int & int))) (resexn (bool & int)) #(witnessable_resexn (bool & int) #(witnessable_pair bool int))) _ =
-//   exportable_arrow a3p _ _ Leaf Leaf _ _
+instance player_args a3p : poly_iface a3p ((int & int) & (mk_poly_arrow a3p int cmp)) =
+  poly_iface_pair a3p (int & int) (mk_poly_arrow a3p int cmp) #_ #(poly_iface_arrow a3p int cmp)
+
+let cb_spec (a3p:threep) : pck_spec =
+  Spec00 true
+    int
+    (witnessable_int)
+    (pre_poly_arrow a3p)
+    cmp
+    (witnessable_cmp)
+    (fun _ -> post_poly_arrow a3p)
+
+let player_spec (a3p:threep) : pck_spec =
+  Spec10 false
+    ((int & int) & (guess: (mk_poly_arrow a3p int cmp)))
+    (witnessable_pair _ _ #(witnessable_pair _ _ #witnessable_int #witnessable_int) #(witnessable_arrow int cmp _ _))
+    (fun x h0 -> inv a3p h0 /\ fst (fst x) < snd (fst x))
+    int
+    witnessable_int
+    (fun _ h0 _ h1 -> inv a3p h1 /\ hrel a3p h0 h1)
+
+(** Stuck here: **)
+instance importable_player (a3p:threep) : safe_importable_to a3p (player_type a3p) (Node (player_spec a3p) Leaf Leaf) =
+  safe_importable_arrow_safe10 
+    a3p _ _
+    #(poly_iface_is_exportable a3p _ #(poly_iface_pair a3p _ _ #(poly_iface_pair a3p int int) #(poly_iface_arrow a3p _ _ #(poly_iface_int a3p) #(poly_iface_cmp a3p))))
+    // #(exportable_pair a3p 
+    //   (int & int) 
+    //   (mk_poly_arrow a3p int cmp) 
+    //   _ _ 
+    //   #(exportable_pair a3p int int Leaf Leaf #(exportable_int a3p) #(exportable_int a3p))
+    //   #(exportable_arrow_no_err00 a3p int _ #(poly_iface_is_safely_importable a3p int) cmp _ #(poly_iface_is_exportable a3p cmp #(poly_iface_cmp a3p)) _ _))
+    _ _ #(poly_iface_is_safely_importable a3p int #(poly_iface_int a3p))
+    (fun x h0 -> inv a3p h0 /\ fst (fst x) < snd (fst x))
+    (fun _ h0 _ h1 -> inv a3p h1 /\ hrel a3p h0 h1)
+
+instance args_importable a3p : importable_to a3p (player_type a3p & (int & (int & int))) _ =
+  importable_pair a3p (player_type a3p) (int & (int & int)) _ Leaf #(safe_importable_is_importable a3p _ _ #(importable_player a3p))
+
+instance exportable_play_guess a3p : exportable_from a3p (play_guess_type a3p) _ =
+  exportable_arrow10 a3p 
+    _ _ _ _ 
+    #(args_importable a3p)
+    #(exportable_resexn a3p (bool & int) (EmptyNode Leaf Leaf) #(exportable_pair a3p bool int Leaf Leaf))
+    _ _
+
